chore: add read/write interfaces to virtual registers

Arm/State.lean
@@ -160,14 +160,23 @@ deriving Repr
 -- General-purpose registers --
 
 -- Read the `idx`-th GPR (with idx = 31 indexing the SP).
--- TODO: Generalize this to read from virtual registers.
 def read_base_gpr (idx : BitVec 5) (s : ArmState) : BitVec 64 :=
   read_store ↑idx s.gpr
+
+-- Read the `idx`-th virtual GPR.
+def read_base_gprv (idx : Nat) (s : ArmState) : BitVec 64 :=
+  read_store (VReg.virtual idx) s.gpr
 
 -- Write `val` to the `idx`-th GPR (with idx = 31 indexing the SP).
 def write_base_gpr (idx : BitVec 5) (val : BitVec 64) (s : ArmState)
   : ArmState :=
     let new_gpr := write_store ↑idx val s.gpr
+    { s with gpr := new_gpr }
+
+-- Write `val` to the `idx`-th virtual GPR
+def write_base_gprv (idx : Nat) (val : BitVec 64) (s : ArmState)
+  : ArmState :=
+    let new_gpr := write_store (VReg.virtual idx) val s.gpr
     { s with gpr := new_gpr }
 
 -- SIMD/FP Registers --
@@ -239,6 +248,7 @@ open BitVec
 
 inductive StateField where
   | GPR    : BitVec 5 → StateField
+  | GPRV   : Nat → StateField -- virtual register for GPR
   | SFP    : BitVec 5 → StateField
   | PC     : StateField
   | FLAG   : PFlag → StateField
@@ -247,6 +257,7 @@ deriving DecidableEq, Repr
 
 -- Injective Lemmas for StateField
 attribute [state_simp_rules] StateField.GPR.injEq
+attribute [state_simp_rules] StateField.GPRV.injEq
 attribute [state_simp_rules] StateField.SFP.injEq
 attribute [state_simp_rules] StateField.FLAG.injEq
 
@@ -254,6 +265,7 @@ def state_value (fld : StateField) : Type :=
   open StateField in
   match fld with
   | GPR _   => BitVec 64
+  | GPRV _   => BitVec 64
   | SFP _   => BitVec 128
   | PC      => BitVec 64
   | FLAG _  => BitVec 1
@@ -264,6 +276,7 @@ def r (fld : StateField) (s : ArmState) : (state_value fld) :=
   open StateField in
   match fld with
   | GPR i   => read_base_gpr i s
+  | GPRV i   => read_base_gprv i s
   | SFP i   => read_base_sfp i s
   | PC      => read_base_pc s
   | FLAG i  => read_base_flag i s
@@ -274,6 +287,7 @@ def w (fld : StateField) (v : (state_value fld)) (s : ArmState) : ArmState :=
   open StateField in
   match fld with
   | GPR i  => write_base_gpr i v s
+  | GPRV i  => write_base_gprv i v s
   | SFP i  => write_base_sfp i v s
   | PC     => write_base_pc v s
   | FLAG i => write_base_flag i v s
@@ -283,6 +297,7 @@ def w (fld : StateField) (v : (state_value fld)) (s : ArmState) : ArmState :=
 theorem r_of_w_same : r fld (w fld v s) = v := by
   unfold r w
   unfold read_base_gpr write_base_gpr
+  unfold read_base_gprv write_base_gprv
   unfold read_base_sfp write_base_sfp
   unfold read_base_pc write_base_pc
   unfold read_base_flag write_base_flag
@@ -294,6 +309,7 @@ theorem r_of_w_different (h : fld1 ≠ fld2) :
   r fld1 (w fld2 v s) = r fld1 s := by
   unfold r w
   unfold read_base_gpr write_base_gpr
+  unfold read_base_gprv write_base_gprv
   unfold read_base_sfp write_base_sfp
   unfold read_base_pc write_base_pc
   unfold read_base_flag write_base_flag
@@ -305,6 +321,7 @@ theorem r_of_w_different (h : fld1 ≠ fld2) :
 theorem w_of_w_shadow : w fld v2 (w fld v1 s) = w fld v2 s := by
   unfold w
   unfold write_base_gpr
+  unfold write_base_gprv
   unfold write_base_sfp
   unfold write_base_pc
   unfold write_base_flag
@@ -315,6 +332,7 @@ theorem w_of_w_shadow : w fld v2 (w fld v1 s) = w fld v2 s := by
 theorem w_irrelevant : w fld (r fld s) s = s := by
   unfold r w
   unfold read_base_gpr write_base_gpr
+  unfold read_base_gprv write_base_gprv
   unfold read_base_sfp write_base_sfp
   unfold read_base_pc write_base_pc
   unfold read_base_flag write_base_flag
@@ -325,6 +343,7 @@ theorem w_irrelevant : w fld (r fld s) s = s := by
 theorem fetch_inst_of_w : fetch_inst addr (w fld val s) = fetch_inst addr s := by
   unfold fetch_inst w
   unfold write_base_gpr
+  unfold write_base_gprv
   unfold write_base_sfp
   unfold write_base_pc
   unfold write_base_flag
@@ -337,6 +356,7 @@ theorem w_program : (w fld v s).program = s.program := by
   intros
   cases fld <;> unfold w <;> simp
   · unfold write_base_gpr; simp
+  · unfold write_base_gprv; simp
   · unfold write_base_sfp; simp
   · unfold write_base_pc; simp
   · unfold write_base_flag; simp
